---
layout: post

---
Day 3

NOTATION  
$$n!$$ is read as n factorian and is defined as:  
$$n!=(n)(n-1)(n-2)\cdots\cdots(2)(1)$$  
and $$0!=1$$  
where n is a non-negative integer.  

RECALL THAT:
The number of sequences of k objects chosen from a collection of n objects, where each object may be used just once is: $$(n)(n-1)(n-2)\cdots\cdots(n-k+1)$$  
But  
$$(n)(n-1)(n-2)\cdots\cdots(n-k+1)=\frac{(n)(n-1)(n-2)\cdots\cdots(n-k+1)(n-k)(n-k-1)\cdots\cdots(1)}{(n-k)(n-k-1)\cdots\cdots(1)}$$  
$$=\frac{n!}{(n-k)!}$$  

THE SUBTRACTION PRINCIPLE  
Suppose again that we have a collection of objects.  
 
$$\#\,of\,objects\,that\,satisfy\,some\,condition$$

$$=total\,\#\,of\,objects-\#\,that\,dont\,satisfy\,the\,condition$$

where \# is read as number

After Day 3, our take away message is:  
<span style="color:blue">$$n!=(n)(n-1)(n-2)\cdots\cdots(2)(1)$$</span>     
<span style="color:blue">$$(n)(n-1)(n-2)\cdots\cdots(n-k+1)=\frac{n!}{(n-k)!}$$</span>     
<span style="color:blue">THE SUBTRACTION PRINCIPLE</span>    